src/tools/parallelcomposition/translateTosapic/sbir_treeScript.sml
@@ -234,7 +234,7 @@ val execute_symbolic_tree_def =
 Define`execute_symbolic_tree tre Eve tre' =
 (case Eve of
    [] => (tre = tre')
- | (e::ev) => (∃tre''. (execute_symbolic_tree tre'' ev tre') ∧ (single_step_execute_symbolic_tree tre e tre''))
+ | (e::ev) => (∃tre''. (execute_symbolic_tree tre ev tre'') ∧ (single_step_execute_symbolic_tree tre'' e tre'))
 )
 `;
 
